theories/effects/io_tape.v
@@ -1,0 +1,144 @@
+(** I/O on a tape effect *)
+From gitrees Require Import prelude gitree.
+
+Record state := State {
+                   inputs : list nat;
+                   outputs : list nat;
+                 }.
+#[export] Instance state_inhabited : Inhabited state := populate (State [] []).
+
+Definition update_input (s : state) : nat * state :=
+  match s.(inputs) with
+  | [] => (0, s)
+  | n::ns =>
+      (n, {| inputs := ns; outputs := s.(outputs) |})
+  end.
+Definition update_output (n:nat) (s : state) : state :=
+  {| inputs := s.(inputs); outputs := n::s.(outputs) |}.
+
+Notation stateO := (leibnizO state).
+
+Program Definition inputE : opInterp :=
+  {|
+    Ins := unitO;
+    Outs := natO;
+  |}.
+
+Program Definition outputE : opInterp :=
+  {|
+    Ins := natO;
+    Outs := unitO;
+  |}.
+
+Definition ioE := @[inputE;outputE].
+
+(* INPUT *)
+Definition reify_input X `{Cofe X} : unitO * stateO →
+                                      option (natO * stateO) :=
+    λ '(o, σ), Some (update_input σ : prodO natO stateO).
+#[export] Instance reify_input_ne X `{Cofe X} :
+  NonExpansive (reify_input X).
+Proof.
+  intros ?[[]][[]][_?]. simpl in *. f_equiv.
+  repeat f_equiv. done.
+Qed.
+
+(* OUTPUT *)
+Definition reify_output X `{Cofe X} : (natO * stateO) →
+                                       option (unitO * stateO) :=
+  λ '(n, σ), Some((), update_output n σ : stateO).
+#[export] Instance reify_output_ne X `{Cofe X} :
+  NonExpansive (reify_output X).
+Proof.
+  intros ?[][][]. simpl in *.
+  repeat f_equiv; done.
+Qed.
+
+Canonical Structure reify_io : sReifier NotCtxDep.
+Proof.
+  simple refine {| sReifier_ops := ioE;
+                   sReifier_state := stateO
+                |}.
+  intros X HX op.
+  destruct op as [[] | [ | []]]; simpl.
+  - simple refine (OfeMor (reify_input X)).
+  - simple refine (OfeMor (reify_output X)).
+Defined.
+
+Section constructors.
+  Context {E : opsInterp} {A} `{!Cofe A}.
+  Context {subEff0 : subEff ioE E}.
+  Context {subOfe0 : SubOfe natO A}.
+  Notation IT := (IT E A).
+  Notation ITV := (ITV E A).
+
+  Program Definition INPUT : (nat -n> IT) -n> IT := λne k, Vis (E:=E) (subEff_opid (inl ()))
+                                                             (subEff_ins (F:=ioE) (op:=(inl ())) ())
+                                                             (NextO ◎ k ◎ (subEff_outs (F:=ioE) (op:=(inl ())))^-1).
+  Solve Obligations with solve_proper.
+  Program Definition OUTPUT_ : nat -n> IT -n> IT :=
+    λne m α, Vis (E:=E) (subEff_opid (inr (inl ())))
+                        (subEff_ins (F:=ioE) (op:=(inr (inl ()))) m)
+                        (λne _, NextO α).
+  Solve All Obligations with solve_proper_please.
+  Program Definition OUTPUT : nat -n> IT := λne m, OUTPUT_ m (Ret 0).
+
+  Lemma hom_INPUT k f `{!IT_hom f} : f (INPUT k) ≡ INPUT (OfeMor f ◎ k).
+  Proof.
+    unfold INPUT.
+    rewrite hom_vis/=. repeat f_equiv.
+    intro x. cbn-[laterO_map]. rewrite laterO_map_Next.
+    done.
+  Qed.
+  Lemma hom_OUTPUT_ m α f `{!IT_hom f} : f (OUTPUT_ m α) ≡ OUTPUT_ m (f α).
+  Proof.
+    unfold OUTPUT.
+    rewrite hom_vis/=. repeat f_equiv.
+    intro x. cbn-[laterO_map]. rewrite laterO_map_Next.
+    done.
+  Qed.
+
+End constructors.
+
+Section weakestpre.
+  Context {sz : nat}.
+  Variable (rs : gReifiers NotCtxDep sz).
+  Context {subR : subReifier reify_io rs}.
+  Notation F := (gReifiers_ops rs).
+  Context {R} `{!Cofe R}.
+  Context `{!SubOfe natO R}.
+  Notation IT := (IT F R).
+  Notation ITV := (ITV F R).
+  Context `{!invGS Σ, !stateG rs R Σ}.
+  Notation iProp := (iProp Σ).
+
+  Lemma wp_input (σ σ' : stateO) (n : nat) (k : natO -n> IT) Φ s :
+    update_input σ = (n, σ') →
+    has_substate σ -∗
+    ▷ (£ 1 -∗ has_substate σ' -∗ WP@{rs} (k n) @ s {{ Φ }}) -∗
+    WP@{rs} (INPUT k) @ s {{ Φ }}.
+  Proof.
+    intros Hs. iIntros "Hs Ha".
+    unfold INPUT. simpl.
+    iApply (wp_subreify_ctx_indep with "Hs").
+    { simpl. rewrite Hs//=. }
+    { simpl. by rewrite ofe_iso_21. }
+    iModIntro. done.
+  Qed.
+
+  Lemma wp_output (σ σ' : stateO) (n : nat) Φ s :
+    update_output n σ = σ' →
+    has_substate σ -∗
+    ▷ (£ 1 -∗ has_substate σ' -∗ Φ (RetV 0)) -∗
+    WP@{rs} (OUTPUT n) @ s {{ Φ }}.
+  Proof.
+    intros Hs. iIntros "Hs Ha".
+    unfold OUTPUT. simpl.
+    iApply (wp_subreify_ctx_indep rs with "Hs").
+    { simpl. by rewrite Hs. }
+    { simpl. done. }
+    iModIntro. iIntros "H1 H2".
+    iApply wp_val. by iApply ("Ha" with "H1 H2").
+  Qed.
+
+End weakestpre.
